coq/Basic/TypeSystem/DType.v
@@ -1,0 +1,61 @@
+(*
+ * Copyright 2015-2016 IBM Corporation
+ *
+ * Licensed under the Apache License, Version 2.0 (the "License");
+ * you may not use this file except in compliance with the License.
+ * You may obtain a copy of the License at
+ *
+ * http://www.apache.org/licenses/LICENSE-2.0
+ *
+ * Unless required by applicable law or agreed to in writing, software
+ * distributed under the License is distributed on an "AS IS" BASIS,
+ * WITHOUT WARRANTIES OR CONDITIONS OF ANY KIND, either express or implied.
+ * See the License for the specific language governing permissions and
+ * limitations under the License.
+ *)
+
+Section DType.
+  Require Import String.
+  Require Import List.
+  Require Import Sorting.
+  Require Import Eqdep_dec.
+  Require Import Bool.
+  Require Import EquivDec Morphisms.
+  
+  Require Import BrandRelation.
+  Require Import ForeignType.
+          
+  Require Import Utils.
+  Require Import RType.
+
+  Context {ftype:foreign_type}.
+  Context {br:brand_relation}.
+
+  (* Note: Tdistr τ is a distributed *collection* of elements with type τ *)
+  Inductive drtype : Set :=
+  | Tlocal : rtype -> drtype
+  | Tdistr : rtype -> drtype.
+  
+  (* Equality is decidable for rtype₀ *)
+  Global Instance drtype_eqdec : EqDec drtype eq.
+  Proof.
+    red; intros.
+    destruct x; destruct y.
+    - destruct (r == r0); unfold equiv, complement in *; subst.
+      * left; reflexivity.
+      * right; congruence.
+    - right; congruence.
+    - right; congruence.
+    - destruct (r == r0); unfold equiv, complement in *; subst.
+      * left; reflexivity.
+      * right; congruence.
+  Qed.
+
+End DType.
+
+    
+(* 
+*** Local Variables: ***
+*** coq-load-path: (("../../../coq" "QCert")) ***
+*** End: ***
+ *)
